prove SUE supply traversal invariants

venom/passes/single_use_expansion/proofs/singleUseExpansionSupplyProofsScript.sml
@@ -4,7 +4,7 @@
 
 Theory singleUseExpansionSupplyProofs
 Ancestors
-  singleUseExpansionDefs irSupply
+  singleUseExpansionDefs irSupply venomInst
 
 (* unit_ir_vars is an occurrence collector (definitions and uses), so it is
    deliberately not ALL_DISTINCT after a generated ASSIGN feeds the rewritten
@@ -47,4 +47,538 @@ Proof
    ir_supply_inst_ok s'` by
     metis_tac[fresh_inst_id_contract] >>
   gvs[]
+QED
+
+
+Definition sue_supply_extends_def:
+  sue_supply_extends s s' <=>
+    ?new_vars new_ids.
+      s'.irs_used_vars = new_vars ++ s.irs_used_vars /\
+      ALL_DISTINCT new_vars /\
+      EVERY (\v. ~MEM v s.irs_used_vars) new_vars /\
+      s'.irs_used_inst_ids = new_ids ++ s.irs_used_inst_ids /\
+      ALL_DISTINCT new_ids /\
+      EVERY (\id. ~MEM id s.irs_used_inst_ids) new_ids /\
+      ir_supply_inst_ok s'
+End
+
+Theorem sue_supply_extends_refl:
+  ir_supply_inst_ok s ==> sue_supply_extends s s
+Proof
+  simp[sue_supply_extends_def] >> metis_tac[]
+QED
+
+Theorem sue_supply_extends_members:
+  sue_supply_extends s s' ==>
+  (!v. MEM v s.irs_used_vars ==> MEM v s'.irs_used_vars) /\
+  (!id. MEM id s.irs_used_inst_ids ==> MEM id s'.irs_used_inst_ids)
+Proof
+  strip_tac >> gvs[sue_supply_extends_def]
+QED
+
+Theorem sue_supply_extends_trans:
+  sue_supply_extends s s1 /\ sue_supply_extends s1 s2 ==>
+  sue_supply_extends s s2
+Proof
+  simp[sue_supply_extends_def] >>
+  rpt strip_tac >>
+  qexistsl [`new_vars' ++ new_vars`,`new_ids' ++ new_ids`] >>
+  gvs[listTheory.ALL_DISTINCT_APPEND, listTheory.EVERY_MEM] >>
+  simp[listTheory.APPEND_ASSOC] >> metis_tac[]
+QED
+
+Theorem sue_alloc_assign_supply_extends:
+  ir_supply_inst_ok s /\ sue_alloc_assign_supply s op = (a,newop,s') ==>
+  sue_supply_extends s s'
+Proof
+  strip_tac >> drule_all sue_alloc_assign_supply_contract >>
+  strip_tac >>
+  simp[sue_supply_extends_def] >> metis_tac[]
+QED
+
+
+Theorem sue_expand_ops_supply_extends:
+  !dfg inst s ops op_idx assigns new_ops s'.
+    ir_supply_inst_ok s /\
+    sue_expand_ops_supply dfg inst s ops op_idx = (assigns,new_ops,s') ==>
+    sue_supply_extends s s'
+Proof
+  Induct_on `ops` >> rpt strip_tac
+  >- gvs[sue_expand_ops_supply_def, sue_supply_extends_refl]
+  >> Cases_on `sue_expand_ops_supply dfg inst s ops (op_idx + 1)` >>
+  PairCases_on `r` >>
+  rename1 `sue_expand_ops_supply dfg inst s ops (op_idx + 1) =
+           (more_assigns,more_ops,s1)` >>
+  `sue_supply_extends s s1` by metis_tac[] >>
+  `ir_supply_inst_ok s1` by gvs[sue_supply_extends_def] >>
+  Cases_on `~sue_needs_assign dfg inst op_idx`
+  >- gvs[sue_expand_ops_supply_def] >>
+  Cases_on `h`
+  >- (Cases_on `sue_alloc_assign_supply s1 (Lit c)` >>
+      PairCases_on `r` >>
+      gvs[sue_expand_ops_supply_def] >>
+      metis_tac[sue_alloc_assign_supply_extends,
+                sue_supply_extends_trans])
+  >- (Cases_on `LENGTH (dfg_get_uses dfg s'') = 1 /\
+                 sue_count_remaining (Var s'') ops = 0`
+      >- gvs[sue_expand_ops_supply_def]
+      >> Cases_on `sue_alloc_assign_supply s1 (Var s'')` >>
+         PairCases_on `r` >>
+         gvs[sue_expand_ops_supply_def] >>
+         metis_tac[sue_alloc_assign_supply_extends,
+                   sue_supply_extends_trans])
+  >> gvs[sue_expand_ops_supply_def]
+QED
+
+
+Theorem sue_expand_inst_supply_extends:
+  ir_supply_inst_ok s /\ sue_expand_inst_supply dfg s inst = (out,s') ==>
+  sue_supply_extends s s'
+Proof
+  rpt strip_tac >> Cases_on `sue_should_skip inst.inst_opcode`
+  >- gvs[sue_expand_inst_supply_def, sue_supply_extends_refl] >>
+  Cases_on `sue_expand_ops_supply dfg inst s inst.inst_operands 0` >>
+  PairCases_on `r` >>
+  gvs[sue_expand_inst_supply_def] >>
+  metis_tac[sue_expand_ops_supply_extends]
+QED
+
+Theorem sue_expand_insts_supply_extends:
+  !dfg s insts outs s'.
+    ir_supply_inst_ok s /\
+    sue_expand_insts_supply dfg s insts = (outs,s') ==>
+    sue_supply_extends s s'
+Proof
+  Induct_on `insts` >> rpt strip_tac
+  >- gvs[sue_expand_insts_supply_def, sue_supply_extends_refl] >>
+  Cases_on `sue_expand_inst_supply dfg s h` >>
+  rename1 `sue_expand_inst_supply dfg s h = (head_out,s1)` >>
+  Cases_on `sue_expand_insts_supply dfg s1 insts` >>
+  rename1 `sue_expand_insts_supply dfg s1 insts = (tail_out,s2)` >>
+  gvs[sue_expand_insts_supply_def] >>
+  `sue_supply_extends s s1` by metis_tac[sue_expand_inst_supply_extends] >>
+  `ir_supply_inst_ok s1` by gvs[sue_supply_extends_def] >>
+  `sue_supply_extends s1 s'` by metis_tac[] >>
+  metis_tac[sue_supply_extends_trans]
+QED
+
+Theorem sue_expand_block_supply_extends:
+  ir_supply_inst_ok s /\ sue_expand_block_supply dfg s bb = (bb',s') ==>
+  sue_supply_extends s s'
+Proof
+  rpt strip_tac >>
+  Cases_on `sue_expand_insts_supply dfg s bb.bb_instructions` >>
+  gvs[sue_expand_block_supply_def] >>
+  metis_tac[sue_expand_insts_supply_extends]
+QED
+
+Theorem sue_expand_blocks_supply_extends:
+  !dfg s bbs bbs' s'.
+    ir_supply_inst_ok s /\
+    sue_expand_blocks_supply dfg s bbs = (bbs',s') ==>
+    sue_supply_extends s s'
+Proof
+  Induct_on `bbs` >> rpt strip_tac
+  >- gvs[sue_expand_blocks_supply_def, sue_supply_extends_refl] >>
+  Cases_on `sue_expand_block_supply dfg s h` >>
+  rename1 `sue_expand_block_supply dfg s h = (bb1,s1)` >>
+  Cases_on `sue_expand_blocks_supply dfg s1 bbs` >>
+  rename1 `sue_expand_blocks_supply dfg s1 bbs = (bbs1,s2)` >>
+  gvs[sue_expand_blocks_supply_def] >>
+  `sue_supply_extends s s1` by metis_tac[sue_expand_block_supply_extends] >>
+  `ir_supply_inst_ok s1` by gvs[sue_supply_extends_def] >>
+  `sue_supply_extends s1 s'` by metis_tac[] >>
+  metis_tac[sue_supply_extends_trans]
+QED
+
+Theorem sue_expand_function_supply_extends:
+  ir_supply_inst_ok s /\ sue_expand_function_supply s fn = (fn',s') ==>
+  sue_supply_extends s s'
+Proof
+  rpt strip_tac >>
+  Cases_on `sue_expand_blocks_supply (dfg_build_function fn) s fn.fn_blocks` >>
+  gvs[sue_expand_function_supply_def] >>
+  metis_tac[sue_expand_blocks_supply_extends]
+QED
+
+Theorem sue_expand_functions_supply_extends:
+  !s fns fns' s'.
+    ir_supply_inst_ok s /\
+    sue_expand_functions_supply s fns = (fns',s') ==>
+    sue_supply_extends s s'
+Proof
+  Induct_on `fns` >> rpt strip_tac
+  >- gvs[sue_expand_functions_supply_def, sue_supply_extends_refl] >>
+  Cases_on `sue_expand_function_supply s h` >>
+  rename1 `sue_expand_function_supply s h = (fn1,s1)` >>
+  Cases_on `sue_expand_functions_supply s1 fns` >>
+  rename1 `sue_expand_functions_supply s1 fns = (fns1,s2)` >>
+  gvs[sue_expand_functions_supply_def] >>
+  `sue_supply_extends s s1` by metis_tac[sue_expand_function_supply_extends] >>
+  `ir_supply_inst_ok s1` by gvs[sue_supply_extends_def] >>
+  `sue_supply_extends s1 s'` by metis_tac[] >>
+  metis_tac[sue_supply_extends_trans]
+QED
+
+Theorem sue_expand_context_supply_extends:
+  ir_supply_inst_ok s /\ sue_expand_context_supply s ctx = (ctx',s') ==>
+  sue_supply_extends s s'
+Proof
+  rpt strip_tac >> Cases_on `sue_expand_functions_supply s ctx.ctx_functions` >>
+  gvs[sue_expand_context_supply_def] >>
+  metis_tac[sue_expand_functions_supply_extends]
+QED
+
+Theorem sue_unit_supply_extends:
+  ir_supply_inst_ok s /\ sue_unit_supply s unit = (unit',s') ==>
+  sue_supply_extends s s'
+Proof
+  rpt strip_tac >> Cases_on `sue_expand_context_supply s unit.cu_context` >>
+  gvs[sue_unit_supply_def] >>
+  metis_tac[sue_expand_context_supply_extends]
+QED
+
+
+Theorem sue_supply_extends_all_distinct:
+  sue_supply_extends s s' /\
+  ALL_DISTINCT s.irs_used_vars /\
+  ALL_DISTINCT s.irs_used_inst_ids ==>
+  ALL_DISTINCT s'.irs_used_vars /\
+  ALL_DISTINCT s'.irs_used_inst_ids
+Proof
+  strip_tac >>
+  gvs[sue_supply_extends_def, listTheory.ALL_DISTINCT_APPEND,
+      listTheory.EVERY_MEM] >> metis_tac[]
+QED
+
+
+Theorem sue_alloc_assign_supply_covered:
+  ir_supply_inst_ok s /\
+  EVERY (\v. MEM v s.irs_used_vars) (venomInst$operand_vars [op]) /\
+  sue_alloc_assign_supply s op = (a,newop,s') ==>
+  EVERY (\v. MEM v s'.irs_used_vars)
+    (inst_ir_vars a ++ venomInst$operand_vars [newop]) /\
+  MEM a.inst_id s'.irs_used_inst_ids
+Proof
+  rpt strip_tac >>
+  drule_all sue_alloc_assign_supply_contract >> strip_tac >>
+  gvs[sue_alloc_assign_supply_def, AllCaseEqs(), inst_ir_vars_def,
+      inst_uses_def, operand_vars_def] >>
+  Cases_on `op` >>
+  gvs[venomInstTheory.operand_vars_def, venomInstTheory.operand_var_def]
+QED
+
+
+Theorem sue_expand_ops_supply_covered:
+  !dfg inst s ops op_idx assigns new_ops s'.
+    ir_supply_inst_ok s /\
+    EVERY (\v. MEM v s.irs_used_vars) (venomInst$operand_vars ops) /\
+    sue_expand_ops_supply dfg inst s ops op_idx = (assigns,new_ops,s') ==>
+    EVERY (\v. MEM v s'.irs_used_vars)
+      (FLAT (MAP inst_ir_vars assigns) ++ venomInst$operand_vars new_ops) /\
+    EVERY (\i. MEM i.inst_id s'.irs_used_inst_ids) assigns
+Proof
+  Induct_on `ops`
+  >- (rpt strip_tac >>
+      gvs[sue_expand_ops_supply_def,
+          venomInstTheory.operand_vars_def])
+  >> rpt strip_tac >>
+  Cases_on `sue_expand_ops_supply dfg inst s ops (op_idx + 1)` >>
+  PairCases_on `r` >>
+  rename1 `sue_expand_ops_supply dfg inst s ops (op_idx + 1) =
+           (more_assigns,more_ops,s1)` >>
+  `sue_supply_extends s s1` by
+    metis_tac[sue_expand_ops_supply_extends] >>
+  `ir_supply_inst_ok s1` by gvs[sue_supply_extends_def] >>
+  `EVERY (\v. MEM v s.irs_used_vars) (venomInst$operand_vars ops)` by
+    (Cases_on `h` >>
+     gvs[venomInstTheory.operand_vars_def,
+         venomInstTheory.operand_var_def]) >>
+  `EVERY (\v. MEM v s1.irs_used_vars)
+     (FLAT (MAP inst_ir_vars more_assigns) ++
+      venomInst$operand_vars more_ops) /\
+   EVERY (\i. MEM i.inst_id s1.irs_used_inst_ids) more_assigns` by
+    metis_tac[] >>
+  `!v. MEM v s.irs_used_vars ==> MEM v s1.irs_used_vars` by
+    metis_tac[sue_supply_extends_members] >>
+  `EVERY (\v. MEM v s1.irs_used_vars)
+     (venomInst$operand_vars [h])` by
+    (Cases_on `h` >>
+     gvs[venomInstTheory.operand_vars_def,
+         venomInstTheory.operand_var_def] >>
+     qpat_assum `!v. MEM v s.irs_used_vars ==>
+                      MEM v s1.irs_used_vars`
+       (qspec_then `s''` irule) >> simp[]) >>
+  Cases_on `sue_alloc_assign_supply s1 h` >>
+  PairCases_on `r` >>
+  rename1 `sue_alloc_assign_supply s1 h = (a,newop,s2)` >>
+  `sue_supply_extends s1 s2` by
+    metis_tac[sue_alloc_assign_supply_extends] >>
+  `EVERY (\v. MEM v s2.irs_used_vars)
+     (inst_ir_vars a ++ venomInst$operand_vars [newop]) /\
+   MEM a.inst_id s2.irs_used_inst_ids` by
+    metis_tac[sue_alloc_assign_supply_covered] >>
+  `!v. MEM v s1.irs_used_vars ==> MEM v s2.irs_used_vars` by
+    metis_tac[sue_supply_extends_members] >>
+  `!id. MEM id s1.irs_used_inst_ids ==> MEM id s2.irs_used_inst_ids` by
+    metis_tac[sue_supply_extends_members] >>
+  `EVERY (\i. MEM i.inst_id s2.irs_used_inst_ids) more_assigns` by
+    (gvs[listTheory.EVERY_MEM] >> rpt strip_tac >>
+     qpat_assum `!i. MEM i more_assigns ==>
+                      MEM i.inst_id s1.irs_used_inst_ids`
+       (qspec_then `i` mp_tac) >> simp[] >> strip_tac >>
+     qpat_assum `!id. MEM id s1.irs_used_inst_ids ==>
+                       MEM id s2.irs_used_inst_ids`
+       (qspec_then `i.inst_id` irule) >> simp[]) >>
+  Cases_on `~sue_needs_assign dfg inst op_idx`
+  >- (gvs[sue_expand_ops_supply_def] >>
+      Cases_on `h` >>
+      gvs[venomInstTheory.operand_vars_def,
+          venomInstTheory.operand_var_def]) >>
+  Cases_on `h`
+  >- (gvs[sue_expand_ops_supply_def, listTheory.EVERY_MEM,
+          venomInstTheory.operand_vars_def] >>
+      rpt strip_tac >> Cases_on `venomInst$operand_var newop` >>
+      gvs[] >> metis_tac[])
+  >- (Cases_on `LENGTH (dfg_get_uses dfg s'') = 1 /\
+                 sue_count_remaining (Var s'') ops = 0`
+      >- (gvs[sue_expand_ops_supply_def,
+              venomInstTheory.operand_vars_def,
+              venomInstTheory.operand_var_def])
+      >> gvs[sue_expand_ops_supply_def, listTheory.EVERY_MEM,
+             venomInstTheory.operand_vars_def,
+             venomInstTheory.operand_var_def] >>
+         rpt strip_tac >> Cases_on `venomInst$operand_var newop` >>
+         gvs[] >> metis_tac[])
+  >> gvs[sue_expand_ops_supply_def,
+         venomInstTheory.operand_vars_def,
+         venomInstTheory.operand_var_def] >>
+  gvs[AllCaseEqs()]
+QED
+
+
+Theorem sue_expand_inst_supply_covered:
+  ir_supply_inst_ok s /\
+  EVERY (\v. MEM v s.irs_used_vars) (inst_ir_vars inst) /\
+  MEM inst.inst_id s.irs_used_inst_ids /\
+  sue_expand_inst_supply dfg s inst = (out,s') ==>
+  EVERY (\v. MEM v s'.irs_used_vars) (FLAT (MAP inst_ir_vars out)) /\
+  EVERY (\i. MEM i.inst_id s'.irs_used_inst_ids) out
+Proof
+  rpt strip_tac >> Cases_on `sue_should_skip inst.inst_opcode`
+  >- gvs[sue_expand_inst_supply_def] >>
+  Cases_on `sue_expand_ops_supply dfg inst s inst.inst_operands 0` >>
+  PairCases_on `r` >>
+  rename1 `sue_expand_ops_supply dfg inst s inst.inst_operands 0 =
+           (assigns,new_ops,s1)` >>
+  gvs[sue_expand_inst_supply_def] >>
+  `sue_supply_extends s s'` by
+    metis_tac[sue_expand_ops_supply_extends] >>
+  `EVERY (\v. MEM v s.irs_used_vars)
+     (venomInst$operand_vars inst.inst_operands)` by
+    gvs[inst_ir_vars_def, inst_uses_def, listTheory.EVERY_APPEND] >>
+  `EVERY (\v. MEM v s'.irs_used_vars)
+      (FLAT (MAP inst_ir_vars assigns) ++
+       venomInst$operand_vars new_ops) /\
+   EVERY (\i. MEM i.inst_id s'.irs_used_inst_ids) assigns` by
+    metis_tac[sue_expand_ops_supply_covered] >>
+  `(!v. MEM v s.irs_used_vars ==> MEM v s'.irs_used_vars) /\
+   (!id. MEM id s.irs_used_inst_ids ==> MEM id s'.irs_used_inst_ids)` by
+    metis_tac[sue_supply_extends_members] >>
+  gvs[inst_ir_vars_def, inst_uses_def, listTheory.EVERY_MEM] >>
+  metis_tac[]
+QED
+
+
+Theorem sue_expand_insts_supply_covered:
+  !dfg s insts outs s'.
+    ir_supply_inst_ok s /\
+    EVERY (\v. MEM v s.irs_used_vars)
+      (FLAT (MAP inst_ir_vars insts)) /\
+    EVERY (\i. MEM i.inst_id s.irs_used_inst_ids) insts /\
+    sue_expand_insts_supply dfg s insts = (outs,s') ==>
+    EVERY (\v. MEM v s'.irs_used_vars) (FLAT (MAP inst_ir_vars outs)) /\
+    EVERY (\i. MEM i.inst_id s'.irs_used_inst_ids) outs
+Proof
+  Induct_on `insts`
+  >- simp[sue_expand_insts_supply_def]
+  >> rpt strip_tac >>
+  Cases_on `sue_expand_inst_supply dfg s h` >>
+  rename1 `sue_expand_inst_supply dfg s h = (head_out,s1)` >>
+  Cases_on `sue_expand_insts_supply dfg s1 insts` >>
+  rename1 `sue_expand_insts_supply dfg s1 insts = (tail_out,s2)` >>
+  gvs[sue_expand_insts_supply_def, listTheory.EVERY_APPEND] >>
+  `sue_supply_extends s s1` by
+    metis_tac[sue_expand_inst_supply_extends] >>
+  `ir_supply_inst_ok s1` by gvs[sue_supply_extends_def] >>
+  `EVERY (\v. MEM v s1.irs_used_vars) (FLAT (MAP inst_ir_vars head_out)) /\
+   EVERY (\i. MEM i.inst_id s1.irs_used_inst_ids) head_out` by
+    metis_tac[sue_expand_inst_supply_covered] >>
+  `(!v. MEM v s.irs_used_vars ==> MEM v s1.irs_used_vars) /\
+   (!id. MEM id s.irs_used_inst_ids ==> MEM id s1.irs_used_inst_ids)` by
+    metis_tac[sue_supply_extends_members] >>
+  `EVERY (\v. MEM v s1.irs_used_vars)
+      (FLAT (MAP inst_ir_vars insts)) /\
+   EVERY (\i. MEM i.inst_id s1.irs_used_inst_ids) insts` by
+    (gvs[listTheory.EVERY_MEM] >> metis_tac[]) >>
+  `EVERY (\v. MEM v s'.irs_used_vars) (FLAT (MAP inst_ir_vars tail_out)) /\
+   EVERY (\i. MEM i.inst_id s'.irs_used_inst_ids) tail_out` by
+    metis_tac[] >>
+  `sue_supply_extends s1 s'` by
+    metis_tac[sue_expand_insts_supply_extends] >>
+  `(!v. MEM v s1.irs_used_vars ==> MEM v s'.irs_used_vars) /\
+   (!id. MEM id s1.irs_used_inst_ids ==> MEM id s'.irs_used_inst_ids)` by
+    metis_tac[sue_supply_extends_members] >>
+  gvs[listTheory.EVERY_MEM] >> metis_tac[]
+QED
+
+
+Theorem sue_expand_block_supply_covered:
+  ir_supply_inst_ok s /\
+  EVERY (\v. MEM v s.irs_used_vars) (block_ir_vars bb) /\
+  EVERY (\id. MEM id s.irs_used_inst_ids) (block_ir_inst_ids bb) /\
+  sue_expand_block_supply dfg s bb = (bb',s') ==>
+  EVERY (\v. MEM v s'.irs_used_vars) (block_ir_vars bb') /\
+  EVERY (\id. MEM id s'.irs_used_inst_ids) (block_ir_inst_ids bb')
+Proof
+  rpt strip_tac >>
+  Cases_on `sue_expand_insts_supply dfg s bb.bb_instructions` >>
+  gvs[sue_expand_block_supply_def, block_ir_vars_def,
+      block_ir_inst_ids_def, listTheory.EVERY_MAP] >>
+  metis_tac[sue_expand_insts_supply_covered]
+QED
+
+Theorem sue_expand_blocks_supply_covered:
+  !dfg s bbs bbs' s'.
+    ir_supply_inst_ok s /\
+    EVERY (\v. MEM v s.irs_used_vars)
+      (FLAT (MAP block_ir_vars bbs)) /\
+    EVERY (\id. MEM id s.irs_used_inst_ids)
+      (FLAT (MAP block_ir_inst_ids bbs)) /\
+    sue_expand_blocks_supply dfg s bbs = (bbs',s') ==>
+    EVERY (\v. MEM v s'.irs_used_vars)
+      (FLAT (MAP block_ir_vars bbs')) /\
+    EVERY (\id. MEM id s'.irs_used_inst_ids)
+      (FLAT (MAP block_ir_inst_ids bbs'))
+Proof
+  Induct_on `bbs`
+  >- simp[sue_expand_blocks_supply_def]
+  >> rpt strip_tac >>
+  Cases_on `sue_expand_block_supply dfg s h` >>
+  rename1 `sue_expand_block_supply dfg s h = (bb1,s1)` >>
+  Cases_on `sue_expand_blocks_supply dfg s1 bbs` >>
+  rename1 `sue_expand_blocks_supply dfg s1 bbs = (bbs1,s2)` >>
+  gvs[sue_expand_blocks_supply_def, listTheory.EVERY_APPEND] >>
+  `sue_supply_extends s s1` by
+    metis_tac[sue_expand_block_supply_extends] >>
+  `ir_supply_inst_ok s1` by gvs[sue_supply_extends_def] >>
+  `EVERY (\v. MEM v s1.irs_used_vars) (block_ir_vars bb1) /\
+   EVERY (\id. MEM id s1.irs_used_inst_ids) (block_ir_inst_ids bb1)` by
+    metis_tac[sue_expand_block_supply_covered] >>
+  `(!v. MEM v s.irs_used_vars ==> MEM v s1.irs_used_vars) /\
+   (!id. MEM id s.irs_used_inst_ids ==> MEM id s1.irs_used_inst_ids)` by
+    metis_tac[sue_supply_extends_members] >>
+  `EVERY (\v. MEM v s1.irs_used_vars) (FLAT (MAP block_ir_vars bbs)) /\
+   EVERY (\id. MEM id s1.irs_used_inst_ids)
+      (FLAT (MAP block_ir_inst_ids bbs))` by
+    (gvs[listTheory.EVERY_MEM] >> metis_tac[]) >>
+  `EVERY (\v. MEM v s'.irs_used_vars)
+      (FLAT (MAP block_ir_vars bbs1)) /\
+   EVERY (\id. MEM id s'.irs_used_inst_ids)
+      (FLAT (MAP block_ir_inst_ids bbs1))` by metis_tac[] >>
+  `sue_supply_extends s1 s'` by
+    metis_tac[sue_expand_blocks_supply_extends] >>
+  `(!v. MEM v s1.irs_used_vars ==> MEM v s'.irs_used_vars) /\
+   (!id. MEM id s1.irs_used_inst_ids ==> MEM id s'.irs_used_inst_ids)` by
+    metis_tac[sue_supply_extends_members] >>
+  gvs[listTheory.EVERY_MEM] >> metis_tac[]
+QED
+
+
+Theorem sue_expand_function_supply_covered:
+  ir_supply_inst_ok s /\
+  EVERY (\v. MEM v s.irs_used_vars) (fn_ir_vars fn) /\
+  EVERY (\id. MEM id s.irs_used_inst_ids) (fn_ir_inst_ids fn) /\
+  sue_expand_function_supply s fn = (fn',s') ==>
+  EVERY (\v. MEM v s'.irs_used_vars) (fn_ir_vars fn') /\
+  EVERY (\id. MEM id s'.irs_used_inst_ids) (fn_ir_inst_ids fn')
+Proof
+  rpt strip_tac >>
+  Cases_on `sue_expand_blocks_supply (dfg_build_function fn) s fn.fn_blocks` >>
+  gvs[sue_expand_function_supply_def, fn_ir_vars_def,
+      fn_ir_inst_ids_def] >>
+  metis_tac[sue_expand_blocks_supply_covered]
+QED
+
+Theorem sue_expand_functions_supply_covered:
+  !s fns fns' s'.
+    ir_supply_inst_ok s /\
+    EVERY (\v. MEM v s.irs_used_vars) (FLAT (MAP fn_ir_vars fns)) /\
+    EVERY (\id. MEM id s.irs_used_inst_ids)
+      (FLAT (MAP fn_ir_inst_ids fns)) /\
+    sue_expand_functions_supply s fns = (fns',s') ==>
+    EVERY (\v. MEM v s'.irs_used_vars) (FLAT (MAP fn_ir_vars fns')) /\
+    EVERY (\id. MEM id s'.irs_used_inst_ids)
+      (FLAT (MAP fn_ir_inst_ids fns'))
+Proof
+  Induct_on `fns`
+  >- simp[sue_expand_functions_supply_def]
+  >> rpt strip_tac >>
+  Cases_on `sue_expand_function_supply s h` >>
+  rename1 `sue_expand_function_supply s h = (fn1,s1)` >>
+  Cases_on `sue_expand_functions_supply s1 fns` >>
+  rename1 `sue_expand_functions_supply s1 fns = (fns1,s2)` >>
+  gvs[sue_expand_functions_supply_def, listTheory.EVERY_APPEND] >>
+  `sue_supply_extends s s1` by
+    metis_tac[sue_expand_function_supply_extends] >>
+  `ir_supply_inst_ok s1` by gvs[sue_supply_extends_def] >>
+  `EVERY (\v. MEM v s1.irs_used_vars) (fn_ir_vars fn1) /\
+   EVERY (\id. MEM id s1.irs_used_inst_ids) (fn_ir_inst_ids fn1)` by
+    metis_tac[sue_expand_function_supply_covered] >>
+  `(!v. MEM v s.irs_used_vars ==> MEM v s1.irs_used_vars) /\
+   (!id. MEM id s.irs_used_inst_ids ==> MEM id s1.irs_used_inst_ids)` by
+    metis_tac[sue_supply_extends_members] >>
+  `EVERY (\v. MEM v s1.irs_used_vars) (FLAT (MAP fn_ir_vars fns)) /\
+   EVERY (\id. MEM id s1.irs_used_inst_ids)
+      (FLAT (MAP fn_ir_inst_ids fns))` by
+    (gvs[listTheory.EVERY_MEM] >> metis_tac[]) >>
+  `EVERY (\v. MEM v s'.irs_used_vars) (FLAT (MAP fn_ir_vars fns1)) /\
+   EVERY (\id. MEM id s'.irs_used_inst_ids)
+      (FLAT (MAP fn_ir_inst_ids fns1))` by metis_tac[] >>
+  `sue_supply_extends s1 s'` by
+    metis_tac[sue_expand_functions_supply_extends] >>
+  `(!v. MEM v s1.irs_used_vars ==> MEM v s'.irs_used_vars) /\
+   (!id. MEM id s1.irs_used_inst_ids ==> MEM id s'.irs_used_inst_ids)` by
+    metis_tac[sue_supply_extends_members] >>
+  gvs[listTheory.EVERY_MEM] >> metis_tac[]
+QED
+
+Theorem sue_expand_context_supply_covered:
+  ir_supply_inst_ok s /\
+  EVERY (\v. MEM v s.irs_used_vars)
+    (FLAT (MAP fn_ir_vars ctx.ctx_functions)) /\
+  EVERY (\id. MEM id s.irs_used_inst_ids)
+    (FLAT (MAP fn_ir_inst_ids ctx.ctx_functions)) /\
+  sue_expand_context_supply s ctx = (ctx',s') ==>
+  EVERY (\v. MEM v s'.irs_used_vars)
+    (FLAT (MAP fn_ir_vars ctx'.ctx_functions)) /\
+  EVERY (\id. MEM id s'.irs_used_inst_ids)
+    (FLAT (MAP fn_ir_inst_ids ctx'.ctx_functions))
+Proof
+  rpt strip_tac >> Cases_on `sue_expand_functions_supply s ctx.ctx_functions` >>
+  gvs[sue_expand_context_supply_def] >>
+  metis_tac[sue_expand_functions_supply_covered]
+QED
+
+Theorem sue_unit_supply_covered:
+  ir_supply_inst_ok s /\
+  EVERY (\v. MEM v s.irs_used_vars) (unit_ir_vars unit) /\
+  EVERY (\id. MEM id s.irs_used_inst_ids) (unit_ir_inst_ids unit) /\
+  sue_unit_supply s unit = (unit',s') ==>
+  EVERY (\v. MEM v s'.irs_used_vars) (unit_ir_vars unit') /\
+  EVERY (\id. MEM id s'.irs_used_inst_ids) (unit_ir_inst_ids unit')
+Proof
+  rpt strip_tac >> Cases_on `sue_expand_context_supply s unit.cu_context` >>
+  gvs[sue_unit_supply_def, unit_ir_vars_def, unit_ir_inst_ids_def] >>
+  metis_tac[sue_expand_context_supply_covered]
 QED
